compiler/backend/passes/proofs/state_caseProofScript.sml
@@ -499,6 +499,29 @@ Proof
   \\ irule env_rel_cons \\ fs []
 QED
 
+Definition dest_thunk_ptr_res_rel_def[simp]:
+  dest_thunk_ptr_res_rel BadRef BadRef = T ∧
+  dest_thunk_ptr_res_rel NotThunk NotThunk = T ∧
+  dest_thunk_ptr_res_rel (IsThunk m1 v1) (IsThunk m2 v2) =
+    (m1 = m2 ∧ v_rel v1 v2) ∧
+  dest_thunk_ptr_res_rel _ _ = F
+End
+
+Theorem dest_thunk_ptr_rel:
+  state_rel s1 s2 ∧
+  v_rel v1 v2 ∧
+  dest_thunk_ptr v1 s1 = res1 ⇒
+    ∃res2.
+      dest_thunk_ptr v2 s2 = res2 ∧
+      dest_thunk_ptr_res_rel res1 res2
+Proof
+  rw [oneline dest_thunk_ptr_def, AllCaseEqs()]
+  \\ gvs [Once v_rel_cases]
+  \\ rpt (TOP_CASE_TAC \\ gvs [])
+  \\ gvs [state_rel_def, LIST_REL_EL_EQN, oEL_THM]
+  \\ first_x_assum drule \\ simp [store_rel_def]
+QED
+
 Theorem step_1_forward:
   ∀tr ts tk tr1 ts1 tk1 ss sr sk.
     step_n 1 (tr,ts,tk) = (tr1,ts1,tk1) ∧
@@ -703,15 +726,24 @@ Proof
     \\ first_assum $ irule_at Any \\ fs [])
   >~ [‘ForceMutK’] >-
    (gvs [step]
-    \\ Cases_on ‘ts’ \\ Cases_on ‘ss’
-    \\ gvs [step_res_rel_cases,state_rel_def,LIST_REL_EL_EQN]
-    \\ reverse $ Cases_on ‘n < LENGTH x'’ \\ gvs []
-    >- gvs [state_rel_def,LIST_REL_EL_EQN]
-    \\ IF_CASES_TAC \\ gvs []
-    \\ last_assum $ qspec_then ‘n’ assume_tac
-    \\ Cases_on ‘EL n x’ \\ Cases_on ‘EL n x'’
-    \\ gvs [store_rel_def,store_same_type_def,state_rel_def,LIST_REL_EL_EQN]
-    \\ rw [store_rel_def, EL_LUPDATE])
+    \\ qpat_x_assum ‘_ = (tr1,ts1,tk1')’ mp_tac
+    \\ TOP_CASE_TAC \\ gvs [OPTREL_def] >- simp [step_res_rel_cases]
+    \\ TOP_CASE_TAC \\ gvs []
+    \\ drule_all dest_thunk_ptr_rel \\ gvs []
+    \\ TOP_CASE_TAC \\ gvs []
+    >~ [‘BadRef’] >- rw [step_res_rel_cases]
+    >~ [‘IsThunk’] >- rw [step_res_rel_cases]
+    \\ (
+      rpt strip_tac \\ gvs []
+      \\ ntac 2 (TOP_CASE_TAC \\ gvs [])
+      \\ gvs [state_rel_def, LIST_REL_EL_EQN, EL_LUPDATE] \\ rw []
+      \\ simp [step_res_rel_cases, store_rel_def]
+      \\ qpat_x_assum ‘store_same_type _ _’ mp_tac
+      \\ qpat_x_assum ‘¬store_same_type _ _’ mp_tac
+      \\ simp [store_same_type_def]
+      \\ rpt (TOP_CASE_TAC \\ gvs []) \\ simp [store_rel_def]
+      \\ first_x_assum drule \\ gvs []
+      \\ simp [store_rel_def]))
   \\ rename [‘AppK’]
   \\ reverse (Cases_on ‘tes’) \\ gvs [] \\ gvs [step]
   >- (simp [Once cont_rel_cases, step_res_rel_cases] \\ rw [])
